feat(Normal Modal): StrictLogicalStrong, `𝐒𝟒 <ᴸ 𝐒𝟓`

Logic/Modal/Normal/ModalCube.lean
@@ -11,18 +11,29 @@ import Logic.Modal.Normal.Completeness
 
 namespace LO.Modal.Normal
 
-def LogicStronger (Λ₁ Λ₂ : AxiomSet β) := ∀ (p : Formula β), (⊧ᴹ[(𝔽(Λ₁) : FrameClass β)] p) → (⊧ᴹ[(𝔽(Λ₂) : FrameClass β)] p)
-infix:20 " ⪯ᴸ " => LogicStronger
+def LogicalStrong (Λ₁ Λ₂ : AxiomSet β) := ∀ (p : Formula β), (⊧ᴹ[(𝔽(Λ₁) : FrameClass β)] p) → (⊧ᴹ[(𝔽(Λ₂) : FrameClass β)] p)
+infix:20 " ≤ᴸ " => LogicalStrong
 
-namespace LogicStronger
+namespace LogicalStrong
 
-instance : IsPreorder (AxiomSet β) (· ⪯ᴸ ·) where
-  refl := by simp_all [LogicStronger];
+instance : IsPreorder (AxiomSet β) (· ≤ᴸ ·) where
+  refl := by simp_all [LogicalStrong];
   trans := by intro Λ₁ Λ₂ Λ₃ h₁₂ h₂₃ p hF; exact h₂₃ p (h₁₂ p hF);
 
 variable {α β : Type u}
-variable {Λ₁ Λ₂ : AxiomSet β} (hS : Λ₁ ⪯ᴸ Λ₂)
-variable [DecidableEq β]
+variable {Λ₁ Λ₂ : AxiomSet β}
+variable [Inhabited α] [DecidableEq β]
+
+lemma iff : (Λ₁ ≤ᴸ Λ₂) ↔ (∀ {F : Frame β}, (F ∈ 𝔽(Λ₂) → F ∈ (𝔽(Λ₁)))) := by
+  constructor;
+  . intro h F hF₂ p hp;
+    exact h p (by simp [Formula.FrameClasses]; aesop) F hF₂;
+  . intro h₁ p h₂ F hF₂;
+    exact h₂ F $ h₁ hF₂;
+
+lemma not_iff : ¬(Λ₁ ≤ᴸ Λ₂) ↔ (∃ F ∈ 𝔽(Λ₂), (F : Frame β) ∉ 𝔽(Λ₁)) := by simpa using iff.not
+
+variable (hS : Λ₁ ≤ᴸ Λ₂)
 
 lemma consequence {Γ} {p : Formula β} : (Γ ⊨ᴹ[(𝔽(Λ₂) : FrameClass α)] p) → (Γ ⊨ᴹ[(𝔽(Λ₁) : FrameClass α)] p) := by
   have := hS;
@@ -31,61 +42,119 @@ lemma consequence {Γ} {p : Formula β} : (Γ ⊨ᴹ[(𝔽(Λ₂) : FrameClass �
 lemma deducible (hComp : Completeness Λ₁ (𝔽(Λ₁) : FrameClass α)) {Γ} {p : Formula β} (hd : Γ ⊢ᴹ[Λ₂]! p) : Γ ⊢ᴹ[Λ₁]! p := by
   exact hComp Γ p $ consequence hS $ AxiomSet.ssounds hd;
 
-end LogicStronger
+end LogicalStrong
 
-def LogicStrictStronger (Λ₁ Λ₂ : AxiomSet β) := (Λ₁ ⪯ᴸ Λ₂) ∧ ¬(Λ₂ ⪯ᴸ Λ₁)
-infix:20 " ≺ᴸ " => LogicStrictStronger
+abbrev LogicalStrictStrong (Λ₁ Λ₂ : AxiomSet β) := (Λ₁ ≤ᴸ Λ₂) ∧ ¬(Λ₂ ≤ᴸ Λ₁)
+infix:20 " <ᴸ " => LogicalStrictStrong
 
 namespace LogicStrictStronger
 
-variable {Λ₁ Λ₂ : AxiomSet β} (hS : Λ₁ ≺ᴸ Λ₂)
-variable [DecidableEq β]
+instance : IsStrictOrder (AxiomSet β) (· <ᴸ ·) where
+  irrefl := by simp [LogicalStrong]
+  trans := by
+    simp [LogicalStrictStrong, LogicalStrong];
+    intro Λ₁ Λ₂ Λ₃ h₁₂ _ _ _ h₂₃ y _ _;
+    constructor;
+    . intro p h₁; exact h₂₃ p $ h₁₂ p h₁;
+    . existsi y;
+      constructor;
+      . simpa;
+      . by_contra hn₁;
+        have := h₁₂ y hn₁;
+        contradiction;
 
-/-
-lemma exists_undeducible_formula
-  (hComp₁ : Completeness Λ₁ (𝔽(Λ₁) : FrameClass β))
-  (hComp₂ : Completeness Λ₂ (𝔽(Λ₂) : FrameClass β))
-  {Γ} : ∃ p, ((Γ ⊢ᴹ[Λ₂]! p) ∧ (Γ ⊬ᴹ[Λ₁]! p)) := by
-  by_contra hC;
-  have : ∀ (p : Formula β), (Γ ⊢ᴹ[Λ₂]! p) → (Γ ⊢ᴹ[Λ₁]! p) := by simpa using hC;
-  apply hS.2;
--/
+variable {Λ₁ Λ₂ : AxiomSet β} (hS : Λ₁ <ᴸ Λ₂)
+variable [DecidableEq β]
 
 end LogicStrictStronger
 
-def LogicEquivalence (Λ₁ Λ₂ : AxiomSet β) := (Λ₁ ⪯ᴸ Λ₂) ∧ (Λ₂ ⪯ᴸ Λ₁)
-infix:75 " ≃ᴸ " => LogicEquivalence
+abbrev LogicalEquivalence (Λ₁ Λ₂ : AxiomSet β) := (Λ₁ ≤ᴸ Λ₂) ∧ (Λ₂ ≤ᴸ Λ₁)
+infix:75 " =ᴸ " => LogicalEquivalence
 
-namespace LogicEquivalence
+namespace LogicalEquivalence
 
-instance : IsEquiv (AxiomSet β) (· ≃ᴸ ·) where
-  refl := by simp [LogicEquivalence]; apply IsRefl.refl;
+instance : IsEquiv (AxiomSet β) (· =ᴸ ·) where
+  refl := by simp; apply IsRefl.refl;
   trans := by
-    simp [LogicEquivalence];
+    simp;
     intros _ _ _ h₁₂ h₂₁ h₂₃ h₃₂;
     constructor;
     . exact IsTrans.trans _ _ _ h₁₂ h₂₃;
     . exact IsTrans.trans _ _ _ h₃₂ h₂₁;
   symm := by
-    simp [LogicEquivalence];
+    simp;
     intros;
     constructor <;> simpa;
 
-variable {α₁ α₂ β} [DecidableEq β]
+variable {α₁ α₂ β} [Inhabited α₁] [Inhabited α₂] [DecidableEq β]
 
 lemma deducible
-  {Λ₁ Λ₂ : AxiomSet β} (h : Λ₁ ≃ᴸ Λ₂)
+  {Λ₁ Λ₂ : AxiomSet β} (h : Λ₁ =ᴸ Λ₂)
   (hComp₁ : Completeness Λ₁ (𝔽(Λ₁) : FrameClass α₁))
   (hComp₂ : Completeness Λ₂ (𝔽(Λ₂) : FrameClass α₂))
   {Γ} {p : Formula β} : (Γ ⊢ᴹ[Λ₁]! p) ↔ (Γ ⊢ᴹ[Λ₂]! p) := by
   constructor;
-  . exact LogicStronger.deducible h.2 hComp₂;
-  . exact LogicStronger.deducible h.1 hComp₁;
+  . exact LogicalStrong.deducible h.2 hComp₂;
+  . exact LogicalStrong.deducible h.1 hComp₁;
 
-end LogicEquivalence
+end LogicalEquivalence
 
 variable {α β : Type u} [Inhabited β] [DecidableEq β]
 variable {p : Formula β}
+
+def LogicKT : AxiomSet α := 𝐊 ∪ 𝐓
+notation "𝐊𝐓" => LogicKT
+
+namespace LogicKT
+
+@[simp] lemma subset_K : 𝐊 ⊆ (𝐊𝐓 : AxiomSet α) := by simp [LogicKT]
+@[simp] lemma subset_T : 𝐓 ⊆ (𝐊𝐓 : AxiomSet α) := by simp [LogicKT]
+
+instance FrameClassDefinability : @FrameClassDefinability α β 𝐊𝐓 (λ F => (Reflexive F)) := by
+  intro F;
+  simp [LogicKT, AxiomSetFrameClass.union];
+  have := AxiomK.defines β F;
+  have := AxiomT.defines β F;
+  aesop;
+
+end LogicKT
+
+theorem sstrong_KD_KT : (𝐊𝐃 : AxiomSet (Fin 2)) <ᴸ 𝐊𝐓 := by
+  constructor;
+  . apply LogicalStrong.iff.mpr;
+    intro F hF;
+    obtain hRefl := LogicKT.FrameClassDefinability.mpr hF;
+    apply LogicKD.FrameClassDefinability.mp;
+    exact serial_of_refl hRefl;
+  . apply LogicalStrong.not_iff.mpr;
+    existsi (λ _ w₂ => w₂ = 1);
+    constructor;
+    . apply LogicKD.FrameClassDefinability.mp;
+      simp [Serial];
+    . apply LogicKT.FrameClassDefinability.not.mp;
+      simp [Reflexive]
+      existsi 0;
+      trivial;
+
+theorem sstrong_S4_S5 : (𝐒𝟒 : AxiomSet (Fin 3)) <ᴸ 𝐒𝟓 := by
+  constructor;
+  . apply LogicalStrong.iff.mpr;
+    intro F hF;
+    obtain ⟨hRefl, hEucl⟩ := LogicS5.FrameClassDefinability.mpr hF;
+    apply LogicS4.FrameClassDefinability.mp;
+    constructor;
+    . exact hRefl;
+    . exact trans_of_refl_eucl hRefl hEucl;
+  . apply LogicalStrong.not_iff.mpr;
+    existsi (λ w₁ w₂ => (w₁ = w₂) ∨ (w₁ = 0 ∧ w₂ = 1) ∨ (w₁ = 0 ∧ w₂ = 2));
+    constructor;
+    . apply LogicS4.FrameClassDefinability.mp;
+      simp [Reflexive, Transitive];
+      trivial;
+    . apply LogicS5.FrameClassDefinability.not.mp;
+      simp [Reflexive, Euclidean];
+      existsi 0, 1, 2;
+      trivial;
 
 def LogicKT4B : AxiomSet α := 𝐊 ∪ 𝐓 ∪ 𝟒 ∪ 𝐁
 notation "𝐊𝐓𝟒𝐁" => LogicKT4B
@@ -107,7 +176,7 @@ instance FrameClassDefinability : @FrameClassDefinability α β 𝐊𝐓𝟒𝐁
   aesop;
 
 abbrev CanonicalModel {β} := Normal.CanonicalModel (𝐊𝐓𝟒𝐁 : AxiomSet β)
-theorem Hilbert.completes : Completeness (𝐊𝐓𝟒𝐁 : AxiomSet β) (𝔽((𝐊𝐓𝟒𝐁 : AxiomSet β)) : FrameClass (MaximalConsistentTheory (𝐊𝐓𝟒𝐁 : AxiomSet β))) := by
+theorem Hilbert.completes : @Completeness (MaximalConsistentTheory (𝐊𝐓𝟒𝐁 : AxiomSet β)) β 𝐊𝐓𝟒𝐁 (𝔽((𝐊𝐓𝟒𝐁 : AxiomSet β)) : FrameClass (MaximalConsistentTheory (𝐊𝐓𝟒𝐁 : AxiomSet β))) := by
   apply completeness_def.mpr;
   intro Γ hConsisΓ;
   let ⟨Ω, hΩ⟩ := exists_maximal_consistent_theory hConsisΓ;
@@ -120,31 +189,20 @@ theorem Hilbert.completes : Completeness (𝐊𝐓𝟒𝐁 : AxiomSet β) (𝔽(
 
 end LogicKT4B
 
-theorem equivalent_S5_KT4B : (𝐒𝟓 : AxiomSet β) ≃ᴸ 𝐊𝐓𝟒𝐁 := ⟨
-  by
-    intro p h F hF;
-    exact h F (by
-      have ⟨hRefl, hTrans, hSymm⟩ := LogicKT4B.FrameClassDefinability.mpr hF;
-      apply LogicS5.FrameClassDefinability.mp;
-      exact ⟨
-        by simpa,
-        eucl_of_symm_trans hSymm hTrans,
-      ⟩;
-    ),
-  by
-    intro p h F hF;
-    exact h F (by
-      have ⟨hRefl, hEucl⟩ := LogicS5.FrameClassDefinability.mpr hF;
-      apply LogicKT4B.FrameClassDefinability.mp;
-      exact ⟨
-        by simpa,
-        trans_of_refl_eucl hRefl hEucl,
-        symm_of_refl_eucl hRefl hEucl,
-      ⟩;
-    );
-⟩
+theorem equivalent_S5_KT4B : (𝐒𝟓 : AxiomSet β) =ᴸ 𝐊𝐓𝟒𝐁 := by
+  constructor;
+  . apply LogicalStrong.iff.mpr;
+    intro F hF;
+    obtain ⟨hRefl, hTrans, hSymm⟩ := LogicKT4B.FrameClassDefinability.mpr hF;
+    apply LogicS5.FrameClassDefinability.mp;
+    exact ⟨hRefl, eucl_of_symm_trans hSymm hTrans⟩
+  . apply LogicalStrong.iff.mpr;
+    intro F hF;
+    obtain ⟨hRefl, hEucl⟩ := LogicS5.FrameClassDefinability.mpr hF;
+    apply LogicKT4B.FrameClassDefinability.mp;
+    exact ⟨hRefl, trans_of_refl_eucl hRefl hEucl, symm_of_refl_eucl hRefl hEucl⟩
 
-theorem deducible_equivalent_S5_KT4B {Γ} {p : Formula β} : (Γ ⊢ᴹ[𝐒𝟓]! p) ↔ (Γ ⊢ᴹ[𝐊𝐓𝟒𝐁]! p) :=
-  LogicEquivalence.deducible equivalent_S5_KT4B LogicS5.Hilbert.completes LogicKT4B.Hilbert.completes
+theorem deducible_equivalent_S5_KT4B {Γ} {p : Formula β} : (Γ ⊢ᴹ[𝐒𝟓]! p) ↔ (Γ ⊢ᴹ[𝐊𝐓𝟒𝐁]! p) := by
+  exact LogicalEquivalence.deducible equivalent_S5_KT4B LogicS5.Hilbert.completes LogicKT4B.Hilbert.completes
 
 end LO.Modal.Normal
